src/SlabsCommon.fsti
@@ -238,7 +238,8 @@ val slab_array
     U32.v md_count < U32.v metadata_max)
   (ensures fun r ->
     A.length r = U32.v page_size /\
-    same_base_array r slab_region
+    same_base_array r slab_region /\
+    A.offset (A.ptr_of r) == A.offset (A.ptr_of slab_region) + U32.v md_count * U32.v page_size
   )
 
 val pack_slab_array (#opened:_)
